theories/asubst_base.v
@@ -1,0 +1,159 @@
+From D Require Import prelude.
+
+Module Type Values.
+  Parameter vl: Type.
+  Definition vls := list vl.
+  Declare Instance inh_vl: Inhabited vl.
+  Declare Instance ids_vl: Ids vl.
+  Declare Instance inj_ids: Inj (=) (=@{vl}) ids.
+
+  Declare Instance rename_vl: Rename vl.
+  Declare Instance subst_vl: Subst vl.
+  Declare Instance subst_lemmas_vl: SubstLemmas vl.
+End Values.
+
+Module Sorts (values: Values).
+  Import values.
+
+  Class Sort (s: Type)
+    {inh_s: Inhabited s}
+    {ids_s: Ids s} {ren_s: Rename s} {hsubst_vl_s: HSubst vl s}
+    {hsubst_lemmas_vl_s: HSubstLemmas vl s} := {}.
+
+  Global Instance sort_vls: Sort vls := {}.
+  Global Instance sort_list `{Sort X}: Sort (list X) := {}.
+  Global Instance sort_pair_snd `{Sort X} `{Inhabited A}: Sort (A * X) := {}.
+  Global Instance sort_list_pair_snd `{Sort X} `{Inhabited A}: Sort (list (A * X)) := {}.
+
+  Implicit Types (v: vl) (vs: vls).
+
+  Definition eq_n_s (s1 s2: var → vl) n := ∀ x, x < n → s1 x = s2 x.
+  Global Arguments eq_n_s /.
+
+  Definition to_subst (ρ: vls) : var → vl := foldr (λ v s, v .: s) ids ρ.
+  Definition subst_sigma (σ: vls) (ρ: vls) := σ.|[to_subst ρ].
+
+  Lemma to_subst_nil: to_subst [] = ids.
+  Proof. trivial. Qed.
+
+  Lemma to_subst_cons v ρ : to_subst (v :: ρ) = v .: to_subst ρ.
+  Proof. trivial. Qed.
+  Global Hint Rewrite to_subst_nil to_subst_cons : autosubst.
+
+  Global Typeclasses Opaque to_subst.
+  Global Opaque to_subst.
+
+  Definition push_var (σ: vls) : vls := ids 0 :: σ.|[ren (+1)].
+  Arguments push_var /.
+
+  (** Create an identity environment of the given length. *)
+  Fixpoint idsσ n: vls :=
+    match n with
+    | 0 => []
+    | S n => push_var (idsσ n)
+    end.
+
+  (** [n]-closedness defines when some AST has at most [n] free variables (from [0] to [n - 1]). *)
+  (** Here and elsewhere, we give one definition for values, using [subst], and
+      another for other ASTs, using [hsubst]. *)
+  Definition nclosed_vl (v: vl) n :=
+    ∀ s1 s2, eq_n_s s1 s2 n → v.[s1] = v.[s2].
+
+  Definition nclosed_σ σ n := Forall (λ v, nclosed_vl v n) σ.
+  Global Arguments nclosed_σ /.
+
+  (** Needed by solve_fv_congruence when dealing with binders, such as in fv_vobj and fv_vabs. *)
+  Lemma eq_up s1 s2 n: eq_n_s s1 s2 n → eq_n_s (up s1) (up s2) (S n).
+  Proof.
+    rewrite /up. move => Heq [|x] Hl //=. f_equiv. apply Heq. lia.
+  Qed.
+
+  Definition stail s := ren (+1) >> s.
+  Definition shead (s: var → vl) := s 0.
+
+  Lemma eq_n_s_tails {n s1 s2}: eq_n_s s1 s2 (S n) → eq_n_s (stail s1) (stail s2) n.
+  Proof. rewrite /stail => /= HsEq x Hl.
+    (* XXX Not needed in syn.v, as id_subst equality holds there definitionally: *)
+    (* asimpl. *) rewrite !id_subst.
+    apply HsEq. lia. Qed.
+
+  Lemma eq_n_s_heads {n s1 s2}: eq_n_s s1 s2 n → n > 0 → shead s1 = shead s2.
+  Proof. rewrite /shead => /= HsEq. apply HsEq. Qed.
+
+  Lemma decomp_s_vl v s:
+    v.[s] = v.[up (stail s)].[shead s/].
+  Proof. by rewrite /stail /shead; asimpl. Qed.
+
+  Notation cl_ρ ρ := (nclosed_σ ρ 0).
+
+  Section sort.
+    Context `{Sort X}.
+
+    Implicit Types (x: X).
+
+    Definition nclosed x n :=
+      ∀ s1 s2, eq_n_s s1 s2 n → x.|[s1] = x.|[s2].
+
+    Lemma decomp_s x s:
+      x.|[s] = x.|[up (stail s)].|[shead s/].
+    Proof. rewrite /stail /shead. by asimpl. Qed.
+  End sort.
+
+  (* XXXX rewrite comment *)
+  (** The following ones are "direct" lemmas: deduce that an expression is closed
+      by knowing that its subexpression are closed. *)
+  (** Automated proof for such lemmas. *)
+  Global Ltac solve_fv_congruence :=
+    rewrite /nclosed /nclosed_vl => * /=; repeat (f_equiv; try solve [(idtac + asimpl); auto using eq_up]).
+
+  (** Rewrite thesis with equalities learned from injection, if possible *)
+  Ltac rewritePremises := let H := fresh "H" in repeat (move => H; rewrite ?H {H}).
+
+  (** Finally, a heuristic solver [solve_inv_fv_congruence] to be able to prove
+      such lemmas easily, both here and elsewhere. *)
+
+  Ltac solve_inv_fv_congruence :=
+    let s1 := fresh "s1" in
+    let s2 := fresh "s2" in
+    let HsEq := fresh "HsEq" in
+    let Hfv := fresh "Hfv" in
+    rewrite /nclosed_vl /nclosed /= => Hfv s1 s2 HsEq;
+  (* asimpl is expensive, but sometimes needed when simplification does mistakes.
+    It must also be done after injection because it might not rewrite under Hfv's
+    binders. *)
+    by [ injection (Hfv s1 s2); trivial; by (idtac + asimpl; rewritePremises; reflexivity) |
+        rewrite ?(decomp_s _ s1) ?(decomp_s _ s2) ?(decomp_s_vl _ s1) ?(decomp_s_vl _ s2) (eq_n_s_heads HsEq); last lia;
+        injection (Hfv _ _ (eq_n_s_tails HsEq)); by rewritePremises ].
+
+  Ltac solve_inv_fv_congruence_h Hcl :=
+    move: Hcl; solve_inv_fv_congruence.
+
+  Ltac solve_inv_fv_congruence_auto :=
+    match goal with
+    | Hcl: nclosed ?x ?n |- nclosed _ _ => solve_inv_fv_congruence_h Hcl
+    | Hcl: nclosed_vl ?v ?n |- nclosed _ _ => solve_inv_fv_congruence_h Hcl
+    | Hcl: nclosed ?x ?n |- nclosed_vl _ _ => solve_inv_fv_congruence_h Hcl
+    | Hcl: nclosed_vl ?v ?n |- nclosed_vl _ _ => solve_inv_fv_congruence_h Hcl
+    end.
+
+  Hint Extern 10 => solve_inv_fv_congruence_auto: fv.
+
+  Section sort_list.
+    Context `{Sort X}.
+    Implicit Types (x: X).
+
+    Lemma fv_cons x xs n: nclosed xs n → nclosed x n → nclosed (x :: xs) n.
+    Proof. solve_fv_congruence. Qed.
+
+    Context `{Inhabited A}.
+    Implicit Types (a: A).
+
+    Lemma fv_pair (a: A) (x: X) n: nclosed x n → nclosed (a, x) n.
+    Proof. solve_fv_congruence. Qed.
+  End sort_list.
+
+  Lemma fv_pair_cons `{!Inhabited A} `{Sort X} (a: A) (x: X) xs n: nclosed xs n → nclosed x n → nclosed ((a, x) :: xs) n.
+  Proof.
+    (* solve_fv_congruence. *) (* Works *)
+    intros. by apply fv_cons, fv_pair. Qed.
+End Sorts.
